\documentclass{article}
\title{CSC352 HW6}
\author{Alex Zhang}
\date{Feb 2023}

\textwidth=16.00cm 
\textheight=22.00cm 
\topmargin=0.00cm
\oddsidemargin=0.00cm 
\evensidemargin=0.00cm 
\headheight=0cm 
\headsep=0.5cm
\textheight=610pt

\usepackage{latexsym,array,delarray,amsthm,amssymb,epsfig}
\usepackage{amsmath}

\newcommand{\bmat}[1]{\begin{bmatrix} #1 \end{bmatrix}}
\newcommand{\mat}[1]{\mathbf{#1}}

\let\ds\displaystyle

\begin{document}
\maketitle

\section*{Question 1}
Given that $\tilde{x} = x(1+\varepsilon_x)$, and $\tilde{y} = y(1+\varepsilon_y)$, we can simplify the inequality,
\begin{align}
    \left| \frac{xy-\tilde{x}\tilde{y}}{xy}\right| &\leq (2+\varepsilon)\varepsilon \nonumber \\
    \left| \frac{xy-(xy+xy\varepsilon_x+xy\varepsilon_y+xy\varepsilon_x\varepsilon_y)}{xy}\right| &\leq (2+\varepsilon)\varepsilon \nonumber \\
    \left| \frac{-xy\varepsilon_x-xy\varepsilon_y-xy\varepsilon_x\varepsilon_y}{xy}\right| &\leq (2+\varepsilon)\varepsilon \nonumber \\
    \left| -\varepsilon_x-\varepsilon_y-\varepsilon_x\varepsilon_y\right| &\leq (2+\varepsilon)\varepsilon \nonumber \\
    \left| \varepsilon_x+\varepsilon_y+\varepsilon_x\varepsilon_y\right| &\leq \varepsilon + \varepsilon + \varepsilon^2 \nonumber
\end{align}
\paragraph*{Csae 1:} $\varepsilon = \left|\frac{x-\tilde{x}}{x}\right|$\\
Since $\tilde{x} = x(1+\varepsilon_x)$, $\varepsilon_x = \left|\frac{\tilde{x}-x}{x}\right| =  \left|\frac{x-\tilde{x}}{x}\right| $. Indicate
$\varepsilon = \varepsilon_x$. Because $\varepsilon_x \geq \varepsilon_y$, $\varepsilon_x^2 \geq \varepsilon_x \varepsilon_y$, we can get that,
$$\varepsilon_x + \varepsilon_x + \varepsilon_x^2 \geq \left| \varepsilon_x+\varepsilon_y+\varepsilon_x\varepsilon_y\right| $$
which is the same as the simplified inequality.

\paragraph*{Case 2:} $\varepsilon = \left|\frac{y-\tilde{y}}{y}\right|$\\
Without loss of generality, we can apply the same proof on $\varepsilon_y$ using $\varepsilon_x$'s and it will have the same result. $\blacksquare$



\section*{Question 2}


\section*{Question 3}

\end{document}